\newpage
\section{Appendix}
Here we give the proof of proposition~\ref{prop:g_nonincr}, which states that $g$ is non-increasing in $b$.

\proof
We take the derivative of $g$:
\begin{align*}
g'(b) &= \frac{2(e-\alpha)}{b^3 \alpha} \log\left(1+\frac{b\alpha}{e-\alpha} \right) - \frac{1}{b^2}-\frac{1}{b^2\left(1+\frac{b\alpha}{e-\alpha}\right)} \leq 0 \\
&\iff \frac{2(e-\alpha)}{b \alpha} \log\left(1+\frac{b\alpha}{e-\alpha} \right) \leq 1+\frac{1}{1+\frac{b\alpha}{e-\alpha}} \\
&\iff \frac{2\log(1+x)}{x} \leq 1+\frac{1}{1+x}
\end{align*}
where $x = \frac{b\alpha}{e-\alpha}$, and as $b \in (0,1)$, $x \in (0, \frac{\alpha}{e-\alpha})$. We can see that as $x \rightarrow 0$, the above inequality is an equality. 
We represent the LHS of the above equation as $L(x)$ and RHS as $R(x)$. Next we show that $L(x)$ decreases more quickly than $R(x)$ does for positive $x$, thereby proving the proposition.
First show that in the range of $x$ the following holds true:

\beq
\label{eq:eq00}
\left(2-\frac{1}{1+x}\right)^2 \le 2\log(1+x) + 1
\eeq
To show the above observe that at $x\rightarrow 0$ both the LHS and RHS are equal. And it is easy to show that the derivative of LHS is lower than the derivative of RHS for all $x\ge 0$ as shown.
\begin{align*}
& (1+x) + \frac{1}{1+x} \ge 2\\
\implies & 2 - \frac{1}{1+x} \le 1 + x\\
\implies & \left(2-\frac{1}{1+x}\right)\cdot \frac{1}{1+x} \le 1\\
\implies & 2\cdot \left(2-\frac{1}{1+x}\right)\cdot \left(\frac{1}{1+x}\right)^2 \le \frac{2}{1+x}
\end{align*}
The left hand side is the derivative of the above LHS and right hand side is the derivative of the above RHS.

Now we can rearrange Eq.~\ref{eq:eq00} as follows:
\begin{align*}
& \left(2-\frac{1}{1+x}\right)^2 \le 2\log(1+x) + 1\\
\implies & \left(1 + \frac{x}{1+x}\right)^2 \le 2\log(1+x) + 1\\
\implies & \left(\frac{x}{1+x}\right)^2 + \frac{2x}{1+x} \le 2\log(1+x)\\
\implies & 2\left(\frac{x}{1+x} - \log(1+x)\right) \le - \left(\frac{x}{1+x}\right)^2\\
\implies & \frac{2\left(\frac{x}{1+x} - \log(1+x)\right)}{x^2} \le - \left(\frac{1}{1+x}\right)^2
\end{align*}
The left hand side of above is $L'(x)$ and right hand side is $R'(x)$.

\endproof